tested before the construction of pb

tactic.sml
@@ -224,6 +224,8 @@ fun exists_tac t (G,fl,f) =
         else raise ERR ("exists_tac.inconsist sorts",[sort_of t,s],[t,var(n,s)],[])
       | _ => raise ERR ("exists_tac.goal is not an existential",[],[],[f])
 
+(*TODO: need to generate a var which is not in the body, so the var in the body with name n do not get covered by this*)
+
 fun spec_all_tac (G,fl,f) = 
     case view_form f of
         vQ("!",n,s,b) =>
