predaxioms.sml
@@ -1,4 +1,4 @@
-
+(*
 fun all_distinct l = 
     case l of [] => true
             | h :: ts => if List.exists (fn t => eq_term(t,h)) ts then false
@@ -62,6 +62,7 @@ fun define_fun f =
         val fsyms0 = new_fun nf (sf,(List.map dest_var args))
     in mk_thm essps [] f
     end
+*)
 
 (*definition database*)
 
@@ -82,49 +83,52 @@ val idR = read_axiom "!A B f: A -> B. f o id(A) = f"
 
 val o_assoc = read_axiom "!A.!B.!f: A -> B.!C.!g:B -> C.!D.!h: C -> D.(h o g) o f = h o g o f";
 
-val isone_def = read_axiom "!one.is1(one) <=> !X.!t1x:X->one.t1x =to1(X,one)";
+val to1_def = read_axiom "!one.is1(one) ==> !X.!t1x:X->one.t1x =to1(X,one)";
 
 val const1_def = read_axiom "is1(1)";
 
 val ax1_1 = const1_def |> existsI ("one",mk_ob_sort) one (rapf "is1(one)")
  
-val iszero_def = read_axiom "!zero.is0(zero) <=> !X.!f0x:zero->X.f0x=from0(zero,X)"
+val from0_def = read_axiom "!zero.is0(zero) ==> !X.!f0x:zero->X.f0x=from0(zero,X)"
 
 val const0_def = read_axiom "is0(0)";
 
 val ax1_2 = const0_def |> existsI ("zero",mk_ob_sort) zero (rapf "is0(zero)")
 
-val pr_def = read_axiom "!A.!B.!AB.!p1:AB->A.!p2:AB->B.ispr(p1,p2)<=>!X.!f:X->A.!g:X->B.!fg:X->AB.p1 o fg = f & p2 o fg = g <=> fg = pa(p1,p2,f,g)";
+
+val pr_def = read_axiom "!A.!B.!AB.!p1:AB->A.!p2:AB->B.ispr(p1,p2)<=>!X.!f:X->A.!g:X->B.?fg:X->AB.!fg':X->AB.p1 o fg' = f & p2 o fg' = g <=> fg' = fg";
+
+val pa_def = read_axiom "!A.!B.!AB.!p1:AB->A.!p2:AB->B.ispr(p1,p2)==>!X.!f:X->A.!g:X->B.!fg:X->AB.p1 o fg = f & p2 o fg = g <=> fg = pa(p1,p2,f,g)";
 
 val pr_ex = read_axiom "!A.!B.?AB.?p1:AB->A.?p2:AB->A.ispr(p1,p2)";
 
 val ax1_3 = pr_ex 
 
-val copr_def = read_axiom "!A.!B.!AB.!i1:A->AB.!i2:B->AB.iscopr(i1,i2)<=>!X.!f:A->X.!g:B->X.!fg:AB->X.fg o i1 = f & fg o i2 = g <=> fg = copa(i1,i2,f,g)"
+val copa_def = read_axiom "!A.!B.!AB.!i1:A->AB.!i2:B->AB.iscopr(i1,i2)==>!X.!f:A->X.!g:B->X.!fg:AB->X.fg o i1 = f & fg o i2 = g <=> fg = copa(i1,i2,f,g)"
 
 val copr_ex = read_axiom "!A.!B.?AB.?i1:A->AB.?i2:B->AB.iscopr(i1,i2)";
 
 val ax1_4 = copr_ex
 
-val eq_def = read_axiom "!A.!B.!f:A->B.!g:A->B.!E.!e:E->A.iseq(e,f,g)<=> f o e = g o e & !X.!x:X->A.f o x = g o x ==> (!x0:X->E.e o x0 = x <=> x0 = eqind(e,f,g,x))"
+val eqind_def = read_axiom "!A.!B.!f:A->B.!g:A->B.!E.!e:E->A.iseq(e,f,g)==> f o e = g o e & !X.!x:X->A.f o x = g o x ==> (!x0:X->E.e o x0 = x <=> x0 = eqind(e,f,g,x))"
 
 val eq_ex = read_axiom "!A.!B.!f:A->B.!g:A->B.?E.?e:E->A.iseq(e,f,g)";
 
 val ax1_5 = eq_ex
 
-val coeq_def = read_axiom "!A.!B.!f:A->B.!g:A->B.!cE.!ce:B->cE.iscoeq(ce,f,g)<=> ce o f = ce o g & !X.!x:B->X. x o f = x o g ==> (!x0:cE->X.x0 o ce = x <=> x0 = coeqind(ce,f,g,x))"
+val coeqind_def = read_axiom "!A.!B.!f:A->B.!g:A->B.!cE.!ce:B->cE.iscoeq(ce,f,g)==> ce o f = ce o g & !X.!x:B->X. x o f = x o g ==> (!x0:cE->X.x0 o ce = x <=> x0 = coeqind(ce,f,g,x))"
 
 val coeq_ex = read_axiom "!A.!B.!f:A->B.!g:A->B.?cE.?ce:B->cE.iscoeq(ce,f,g)"
 
 val ax1_6 = coeq_ex
 
-val exp_def = read_axiom "!A.!B.!A2B.!efs.!p1:efs ->A.!p2:efs ->A2B.!ev:efs->B.isexp(p1,p2,ev)<=> ispr(p1,p2) & !X.!AX.!p1':AX->A.!p2':AX->X. ispr(p1',p2') ==> !f:AX->B.!h:X->A2B. ev o pa(p1,p2,p1',h o p2') = f <=> h = tp(p1,p2,ev,p1',p2',f)"
+val tp_def = read_axiom "!A.!B.!A2B.!efs.!p1:efs ->A.!p2:efs ->A2B.!ev:efs->B.isexp(p1,p2,ev)==> ispr(p1,p2) & !X.!AX.!p1':AX->A.!p2':AX->X. ispr(p1',p2') ==> !f:AX->B.!h:X->A2B. ev o pa(p1,p2,p1',h o p2') = f <=> h = tp(p1,p2,ev,p1',p2',f)"
 
 val exp_ex = read_axiom "!A.!B.?A2B efs p1:efs ->A p2:efs ->A2B ev:efs->B.isexp(p1,p2,ev)"
 
 val ax2 = exp_ex
 
-val N0_def = read_axiom "!N0 one z0:one -> N0 s0:N0->N0. isN0(z0,s0) <=> is1(one) & !X x0:one -> X t:X -> X x:N0 -> X. x o z0 = x0 & x o s0 = t o x <=> x = Nind0(z0,s0,x0,t)";
+val Nind0_def = read_axiom "!N0 one z0:one -> N0 s0:N0->N0. isN0(z0,s0) ==> is1(one) & !X x0:one -> X t:X -> X x:N0 -> X. x o z0 = x0 & x o s0 = t o x <=> x = Nind0(z0,s0,x0,t)";
 
 
 val constN_def = read_axiom "!X x0:1->X t:X ->X x:N->X.x o z = x0 & x o s = t o x <=> x = Nind(x0,t)"
@@ -177,7 +181,7 @@ fun disch_all' th = dischl' (ant th) th
 
 fun disch_all'' th = dischl'' (ant th) th
 
-val eq_eqn = eq_def |> iffLR |> strip_all_and_imp
+val eq_eqn = eqind_def |> strip_all_and_imp
                     |> conjE2 |> iffRL |> strip_all_and_imp
                     |> rewr_rule [assume (rapf "x0 = eqind(e:E->A, f:A->B, g, x:X->A)")] |> disch (rapf "x0 = eqind(e:E->A, f:A->B, g, x:X->A)")
                     |> gen_all 
@@ -196,7 +200,7 @@ fun arw_rule thl th = rewr_rule ((List.map assume $ ant th) @ thl) th
 (*∀A B X f. f∶A × X → B ⇒ ev A B ∘ ⟨p1 A X, tp f ∘ p2 A X⟩ = f*)
 
 val ev_of_tp = 
-exp_def |> iffLR |> strip_all_and_imp |> conjE2 |> strip_all_and_imp |> iffRL |>
+tp_def |> strip_all_and_imp |> conjE2 |> strip_all_and_imp |> iffRL |>
 undisch |> arw_rule [] |> disch (rapf "h = tp(p1:efs->A, p2:efs->A2B, ev:efs->B, p1':AX->A, p2':AX->X, f)") |> allI ("h",mk_ar_sort (mk_ob "X") (mk_ob "A2B"))|>
 allE $ rastt "tp(p1:efs->A, p2:efs->A2B, ev:efs->B, p1':AX->A, p2':AX->X, f)"|>
 C mp $ refl $ rastt "tp(p1:efs->A, p2:efs->A2B, ev:efs->B, p1':AX->A, p2':AX->X, f)" |> 
@@ -230,7 +234,7 @@ e0
             (ev A B) o ⟨p1 A X, h o (p2 A X)⟩ = f ⇒
             h = tp f
 *)
-val is_tp = exp_def |> iffLR |> strip_all_and_imp |> conjE2 |> iffLR
+val is_tp = tp_def |> strip_all_and_imp |> conjE2 |> iffLR
                     |> disch_all'' |> gen_all
 
 (*
@@ -240,7 +244,7 @@ val is_tp = exp_def |> iffLR |> strip_all_and_imp |> conjE2 |> iffLR
                  h = tp f)
 *)
 
-val ax2_conj2 = exp_def |> iffLR |> strip_all_and_imp |> conjE2 |> disch_all'' |> gen_all
+val ax2_conj2 = tp_def |> strip_all_and_imp |> conjE2 |> disch_all'' |> gen_all
 
 (*
 ∀X x0 t. x0∶ one → X ∧ t∶ X → X ⇒
@@ -256,7 +260,7 @@ ax3_conj2
             f = g
 *)
 
-val exp_ispr = exp_def |> iffLR |> strip_all_and_imp |> conjE1 |> disch_all |> gen_all
+val exp_ispr = tp_def |> strip_all_and_imp |> conjE1 |> disch_all |> gen_all
 
 
 
@@ -275,17 +279,373 @@ e0
 
 val to_p_component = proved_th $
 e0
-(repeat strip_tac >> match_mp_tac (pr_def |> iffLR |> iffLR |> irule_canon) >>
+(repeat strip_tac >> match_mp_tac (pa_def |> iffLR |> irule_canon) >>
  arw_tac[])
 (rapg "!A B AB p1:AB->A p2:AB->B. ispr(p1, p2) ==>!X f:X->AB. f = pa(p1, p2, p1 o f, p2 o f)")
 
-val to_p_eq = 
+val to_p_eq = proved_th $
 e0
 (repeat strip_tac >> 
  suffices_tac (rapf "f = pa(p1:AB->A,p2:AB->B,p1 o (f:X->AB),p2 o f) & g = pa(p1:AB->A,p2:AB->B,p1 o (g:X->AB),p2 o g)")
  >-- (strip_tac >> once_arw_tac[] >> arw_tac[]) >> strip_tac
  >> match_mp_tac to_p_component >> arw_tac[])
 (rapg "!A B AB p1:AB->A p2:AB->B.ispr(p1,p2) ==> !X f:X ->AB g. p1 o f = p1 o g & p2 o f = p2 o g ==> f = g ")
+
+val from_copr_components = proved_th $
+e0
+(repeat strip_tac >> match_mp_tac (copa_def |> iffLR |> irule_canon) >>
+arw_tac[])
+(rapg "!A B AB i1:A->AB i2:B->AB. iscopr(i1, i2) ==>!X f:AB->X. f = copa(i1, i2, f o i1, f o i2)")
+
+
+
+(*i1 one one ≠ i2 one one*)
+(*val i1_ne_i2 = proved_th $
+e0
+(repeat strip_tac >> ccontra_tac >> 
+ x_choosel_then ["X","x1","x2"])
+(rapg "!one oneone i1:one -> oneone i2:one -> oneone. is1(one) & iscopr(i1,i2) ==> ~i1 = i2")
+*)
+
+(*∀A B X f g. f∶ A → X ∧ g∶ B → X ⇒ copa f g o i1 A B = f*)
+
+val i12_of_copa = copa_def |> iffRL |> spec_all |> undisch
+                          |> specl (List.map rastt ["X","f:A->X","g:B->X","copa(i1:A->AB,i2:B->AB,f:A->X,g)"]) |> C mp $ refl (rastt "copa(i1:A->AB,i2:B->AB,f:A->X,g)") 
+                          |> gen_all |> disch_all |> gen_all
+                         
+
+val i1_of_copa = copa_def |> iffRL |> spec_all |> undisch
+                          |> specl (List.map rastt ["X","f:A->X","g:B->X","copa(i1:A->AB,i2:B->AB,f:A->X,g)"]) |> C mp $ refl (rastt "copa(i1:A->AB,i2:B->AB,f:A->X,g)") 
+                          |> conjE1 |> gen_all |> disch_all |> gen_all
+
+val i2_of_copa = copa_def |> iffRL |> spec_all |> undisch
+                          |> specl (List.map rastt ["X","f:A->X","g:B->X","copa(i1:A->AB,i2:B->AB,f:A->X,g)"]) |> C mp $ refl (rastt "copa(i1:A->AB,i2:B->AB,f:A->X,g)") 
+                          |> conjE2 |> gen_all |> disch_all |> gen_all
+
+
+
+(*may add once full simp *)
+val i1_ne_i2 = proved_th $
+e0
+(repeat strip_tac >> ccontra_tac >> 
+ x_choosel_then ["X","x1","x2"] assume_tac ax8 >> 
+ by_tac (rapf "copa(i1:1->oneone,i2:1->oneone,x1:1->X,x2) o i1 = x1 &copa(i1,i2,x1,x2) o i2 = x2") >-- (drule i12_of_copa >> arw_tac[]) >>
+ pop_assum (assume_tac o GSYM) >> 
+ rev_full_simp_tac[] >> suffices_tac (rapf "x1:1->X = x2") 
+ >-- (arw_tac[] >> first_assum accept_tac) >>
+ pick_x_assum (rapf "~x1:1->X = x2") (K all_tac) >> once_arw_tac[] >> rw_tac[])
+(rapg "!oneone i1:1 -> oneone i2:1 -> oneone. iscopr(i1,i2) ==> ~i1 = i2")
+
+(*∀A B x. ¬(x∶one → (A + B) ∧ (∃x0 x0'. x0∶one → A ∧ x0'∶one → B ∧
+                             i1 A B ∘ x0 = x ∧
+                             i2 A B ∘ x0' = x))
+*)
+
+(* TODO:  i1_ne_i2|> spec_all |> undisch|> eqF_intro |> iffLR |> disch_all|> gen_all |>irule_canon
+# Exception- ERR ("the given variable occurs unexpectedly", [], [], []) raised
+
+
+*)
+
+val eq_to1 = mp (allE one to1_def) const1_def 
+
+val to1_unique = specl [rastt "X",rastt "f:X->1"] eq_to1 |> GSYM 
+                       |> trans (specl [rastt "X",rastt "g:X->1"] eq_to1) |> gen_all
+
+val prop_5_lemma = proved_th $
+e0
+(repeat strip_tac >> x_choosel_then ["oneone","one1","one2"] assume_tac  (specl (List.map rastt ["1","1"]) copr_ex) >> ccontra_tac >>
+match_mp_tac (i1_ne_i2|> spec_all |> undisch|> eqF_intro |> iffLR |> undisch|> conj_all_assum |> disch_all|> gen_all) >>
+exists_tac (rastt "oneone") >> exists_tac (rastt "one1:1->oneone") >>
+exists_tac (rastt "one2:1->oneone") >> 
+arw_tac[] >> pop_assum mp_tac >> pop_assum mp_tac >> drule i12_of_copa >>
+first_x_assum (specl_then (List.map rastt ["oneone","(one1:1->oneone) o (to1(A,1))",
+                                           "(one2:1->oneone) o (to1(B,1))"]) assume_tac) >>
+repeat strip_tac >>
+suffices_tac (rapf "(one1:1->oneone) o (to1(A,1)) o (x0:1->A) = (one2:1->oneone) o (to1(B,1)) o (x0':1->B)") 
+>-- ((*by_tac (rapf " to1(A, 1) o (x0:1->A) = to1(B, 1) o x0'") TODO: do not understand why cannot use rw to1_unique to solve this by*)
+      assume_tac (specl (List.map rastt ["1","id(1)","to1(A, 1) o (x0:1->A)"]) to1_unique) >>  assume_tac (specl (List.map rastt ["1","id(1)","to1(B, 1) o (x0':1->B)"]) to1_unique)>>
+  arw_tac[] >> rw_tac[idR]) >>
+suffices_tac (rapf "copa(i1:A->AB, i2:B->AB, ((one1:1->oneone) o to1(A, 1)), ((one2:1->oneone) o to1(B, 1))) o i1 o (x0:1->A) = copa(i1, i2, (one1 o to1(A, 1)), (one2 o to1(B, 1))) o i2 o x0'") 
+>-- (rw_tac[GSYM o_assoc] >> arw_tac[]) >>
+arw_tac[]
+)
+(rapg "!A B AB i1:A->AB i2:B->AB. iscopr(i1,i2) ==> !x0:1->A x0':1->B.~i1 o x0 = i2 o x0'")
+
+val from_cop_eq = proved_th $
+e0
+(repeat strip_tac >> 
+ suffices_tac (rapf "f = copa(i1:A->AB,i2:B->AB,(f:AB->X) o i1,f o i2) & g = copa(i1,i2,(g:AB->X) o i1,g o i2)")
+ >-- (strip_tac >> once_arw_tac[] >> arw_tac[]) >> strip_tac
+ >> match_mp_tac from_copr_components >> arw_tac[])
+(rapg "!A B AB i1:A->AB i2:B->AB.iscopr(i1,i2) ==> !X f:AB ->X g. f o i1 = g o i1 & f o i2 = g o i2 ==> f = g ")
+
+(*!X t. t∶ one → X ==> i1 X X o t <> i2 X X o t*)
+
+
+val i1_i2_disjoint = proved_th $
+e0
+(repeat strip_tac >> match_mp_tac prop_5_lemma >> arw_tac[])
+(rapg "!X XX i1:X->XX i2:X->XX. iscopr(i1,i2) ==> !t:1->X. ~i1 o t = i2 o t")
+
+val pr_with_one = proved_th $
+e0
+(strip_tac >> rw_tac[pr_def] >> repeat strip_tac >> exists_tac (rastt "f:X->A") >>
+repeat strip_tac >> dimp_tac (* 2 *)
+>-- (strip_tac >> full_simp_tac[idL]) >>
+strip_tac >> arw_tac[idL] >> rw_tac[specl (List.map rastt ["X","g:X->1"]) to1_unique])
+(rapg "!A. ispr(id(A),to1(A,1))")
+
+(*
+∀A B C D P Q f g i j. f∶ A → C ∧ g∶ B → D ∧ i∶ C → P ∧ j∶ D → Q ⇒
+                      ⟨i o p1 C D,j o p2 C D⟩ o ⟨f o p1 A B, g o p2 A B⟩ =
+                      ⟨i o f o p1 A B, j o g o p2 A B⟩*)
+
+fun dest_form_view fv = case fv of vQ("?",n,s,b) => (n,s,b)
+
+
+
+val p12_of_pa = pa_def |> iffRL |> spec_all |> undisch
+                       |> specl (List.map rastt ["X","f:X->A","g:X->B","pa(p1:AB->A,p2:AB->B,f:X->A,g)"]) |> C mp $ refl (rastt "pa(p1:AB->A,p2:AB->B,f:X->A,g)") 
+                       |> gen_all |> disch_all |> gen_all
+                       
+
+val p1_of_pa =  pa_def |> iffRL |> spec_all |> undisch
+                         |> specl (List.map rastt ["X","f:X->A","g:X->B","pa(p1:AB->A,p2:AB->B,f:X->A,g)"]) |> C mp $ refl (rastt "pa(p1:AB->A,p2:AB->B,f:X->A,g)")                
+                         |> conjE1 |> gen_all |> disch_all |> gen_all
+
+val p2_of_pa =  pa_def |> iffRL |> spec_all |> undisch
+                         |> specl (List.map rastt ["X","f:X->A","g:X->B","pa(p1:AB->A,p2:AB->B,f:X->A,g)"]) |> C mp $ refl (rastt "pa(p1:AB->A,p2:AB->B,f:X->A,g)")                
+                         |> conjE2 |> gen_all |> disch_all |> gen_all
+
+
+(*AQ: massive conditional rw here *)
+
+val parallel_p_compose = proved_th $
+e0
+(strip_tac >> match_mp_tac (irule_canon to_p_eq) >> 
+ exists_tac (rastt "P") >> exists_tac (rastt "Q") >>
+ exists_tac (rastt "pP:PQ->P") >> exists_tac (rastt "pQ:PQ->Q") >> strip_tac (* 2 *)
+ >-- (drule p2_of_pa >> arw_tac[] >> arw_tac[GSYM o_assoc] >> 
+      pick_x_assum (rapf "ispr(pC:CD->C, pD:CD->D)") assume_tac >> 
+      drule p2_of_pa >> arw_tac[o_assoc]) >>
+ drule p1_of_pa >> arw_tac[GSYM o_assoc] >> 
+ pick_x_assum (rapf "ispr(pC:CD->C, pD:CD->D)") assume_tac >> 
+ drule p1_of_pa >> arw_tac[o_assoc]
+ )
+(rapg "ispr(pM:MN->M,pN:MN->N1)& ispr(pC:CD->C,pD:CD->D) & ispr(pP:PQ->P,pQ:PQ->Q) ==> pa(pP,pQ, i o pC,j o pD) o pa(pC,pD,f o pM,g o pN) = pa(pP,pQ,i o f o pM,j o g o pN) ")
+
+
+
+(*
+∀A B C D P Q f g i j. f∶ A → C ∧ g∶ B → D ∧ i∶ C → P ∧ j∶ D → Q ⇒
+                      ⟨i o p1 C D,j o p2 C D⟩ o ⟨f o p1 A B, g o p2 A B⟩ =
+                      ⟨i o f o p1 A B, j o g o p2 A B⟩
+
+(id A)∶A → A ∧ f∶B → C ∧ id A∶ A → A ∧ g∶ C → D ⇒
+   ⟨(id A) ∘ p1 A C, g ∘ p2 A C⟩ ∘ ⟨id A ∘ p1 A B, f ∘ p2 A B⟩ =
+   ⟨(id A) ∘ (id A) ∘ p1 A B,g ∘ f ∘ p2 A B⟩
+
+∀A B C D f g.f∶ B → C ∧ g∶ C→ D ⇒
+             ⟨p1 A B,g o f o p2 A B⟩ =
+             ⟨p1 A C, g o p2 A C⟩ o ⟨p1 A B, f o p2 A B⟩
+*)
+
+val parallel_p_one_side = 
+proved_th $ 
+e0 
+(strip_tac >> by_tac (rapf "ispr(pA:AB ->A,pB:AB->B) & ispr(pA':AC->A,pC:AC->C) & ispr(pA'':AD->A,pD:AD->D)")
+>-- arw_tac[] >> 
+drule (parallel_p_compose |> undisch |> gen_all |> disch_all |> gen_all) >>
+first_x_assum (specl_then (List.map rastt ["id(A)","f:B->C","id(A)","g:C->D"]) assume_tac)>>
+full_simp_tac[idL])
+(rapg "ispr(pA:AB ->A,pB:AB->B) & ispr(pA':AC->A,pC:AC->C) & ispr(pA'':AD->A,pD:AD->D) ==>pa(pA'',pD,pA,(g:C->D) o (f:B->C) o pB) = pa(pA'',pD,pA',g o pC) o pa(pA',pC,pA,f o pB)")
+
+val parallel_p_one_side' = proved_th $
+e0
+(strip_tac >> assume_tac (undisch parallel_p_one_side) >> arw_tac[o_assoc])
+(rapg "ispr(pA:AB ->A,pB:AB->B) & ispr(pA':AC->A,pC:AC->C) & ispr(pA'':AD->A,pD:AD->D) ==>pa(pA'',pD,pA,((g:C->D) o (f:B->C)) o pB) = pa(pA'',pD,pA',g o pC) o pa(pA',pC,pA,f o pB)")
+
+
+(*∀A B C D E f g h.
+         f∶B → C ∧ g∶C → D /\ h ∶ D → E ⇒
+         ⟨p1 A B,(h o g ∘ f) ∘ p2 A B⟩ =
+         ⟨p1 A D, h ∘ p2 A D⟩ o ⟨p1 A C,g ∘ p2 A C⟩ ∘ ⟨p1 A B,f ∘ p2 A B⟩
+*)
+val parallel_p_one_side = parallel_p_one_side |> undisch|> gen_all |> disch_all |> gen_all
+
+val parallel_p_one_side_three = proved_th $
+e0
+(strip_tac >> by_tac (rapf "ispr(pA:AB ->A,pB:AB->B) & ispr(pA'':AD->A,pD:AD->D) & ispr(pA''':AE->A,pE:AE->E)") >-- arw_tac[] >>
+drule parallel_p_one_side >> first_x_assum (specl_then (List.map rastt ["(g:C->D) o (f:B->C)","h:D->E"]) assume_tac) >> full_simp_tac[o_assoc] >>
+suffices_tac (rapf "pa(pA'':AD->A, pD:AD->D, pA:AB->A, (g:C->D) o (f:B->C) o (pB:AB->B)) = pa(pA'', pD, pA':AC->A, (g o pC)) o pa(pA', pC:AC->C, pA, f o pB)")
+>-- (strip_tac >> arw_tac[]) >>
+by_tac (rapf "ispr(pA:AB ->A,pB:AB->B) & ispr(pA':AC->A,pC:AC->C) & ispr(pA'':AD->A,pD:AD->D)") >-- arw_tac[] >> 
+drule parallel_p_one_side >> arw_tac[])
+(rapg "ispr(pA:AB ->A,pB:AB->B) & ispr(pA':AC->A,pC:AC->C) & ispr(pA'':AD->A,pD:AD->D) & ispr(pA''':AE->A,pE:AE->E)==>pa(pA''',pE,pA,(h:D->E) o (g:C->D) o (f:B->C) o pB) = pa(pA''',pE,pA'',h o pD) o pa(pA'',pD,pA',g o pC) o pa(pA',pC,pA,f o pB)")
+
+(*
+∀X A B C f g. (f∶X → ((A×B)×C) ∧ g∶X → ((A×B)×C) ∧ 
+               (p1 A B) o (p1 (A×B) C) o f =  (p1 A B) o (p1 (A×B) C) o g ∧
+               (p2 A B) o (p1 (A×B) C) o f =  (p2 A B) o (p1 (A×B) C) o g ∧
+               (p2 (A×B) C) o f = (p2 (A×B) C) o g) ⇒ f = g
+*)
+
+val iterated_p_eq_applied = proved_th $
+e0
+(repeat strip_tac >> match_mp_tac (irule_canon to_p_eq) >> 
+exists_tac (rastt "PQ") >> exists_tac (rastt "C") >> exists_tac (rastt "pPQ:PQC->PQ") >>
+exists_tac (rastt "pC:PQC->C") >> arw_tac[] >> match_mp_tac (irule_canon to_p_eq) >>
+exists_tac (rastt "P") >> exists_tac (rastt "Q") >> 
+exists_tac (rastt "pP:PQ->P")>> exists_tac (rastt "pQ:PQ->Q") >> arw_tac[])
+(rapg "ispr(pPQ:PQC->PQ,pC:PQC->C) & ispr(pP:PQ->P,pQ:PQ->Q) ==> !X f:X->PQC g. pP o pPQ o f = pP o pPQ o g & pQ o pPQ o f = pQ o pPQ o g & pC o f = pC o g ==> f = g")
+
+
+(*id N = N_ind z s*)
+
+val N_ind_z_s_id = constN_def |> specl (List.map rastt ["N","z","s","id(N)"])
+                              |> rewr_rule [idL,idR]
+
+
+(*∀f. f∶ N → N ∧ f o z = z ∧ f o s = s o f ⇒ f = id N*)
+
+val comm_with_s_id = 
+    constN_def |> specl (List.map rastt ["N","z","s","f:N->N"])
+               |> iffLR |> undisch |> GSYM |> trans N_ind_z_s_id |> disch_all |> gen_all
+
+(*∀A B f g. f∶ A → B ∧ g∶ A → B ∧ ⟨id A,f⟩ = ⟨id A,g⟩ ⇒ f = g*)
+val to_p_components = to_p_component;
+
+
+(*AQ: once_arw_tac[] can cause :  # # # # # Exception- ERR ("extra variable involved", [A -> A], [f], []) raised, how to prevent this?*)
+
+val to_p_eq_one_side = proved_th $
+e0
+(repeat strip_tac >> drule p2_of_pa >> pop_assum (assume_tac o GSYM) >> 
+ first_assum (specl_then (List.map rastt ["A","id(A)","f:A->B"]) assume_tac) >> 
+ first_x_assum (specl_then (List.map rastt ["A","id(A)","g:A->B"]) assume_tac) >>
+ once_arw_tac[] >> pop_assum (K all_tac) >> pop_assum (K all_tac) >> arw_tac[])
+(rapg "ispr(p1:AB ->A,p2:AB->B) ==> !f:A->B g. pa(p1,p2,id(A),f) = pa(p1,p2,id(A),g) ==> f = g")
+
+val _ = new_pred "isinc" [("a",mk_ar_sort (mk_ob "A") (mk_ob "X")),
+                          ("b",mk_ar_sort (mk_ob "B") (mk_ob "X"))]
+
+(*is_inc a b A ⇔ is_subset a A ∧ is_subset b A ∧ ∃h. h∶(dom a) → (dom b) ∧ b o h = a*)
+
+val isinc_def = read_axiom "!X A B a b.isinc(a:A->X,b:B->X) <=> ismono(a) & ismono(b) & ?h:A->B. b o h = a"
+
+val ismono_applied = ismono_def |> iffRL
+
+val ismono_property = ismono_def |> iffLR
+
+
+(*∀A B m i. m∶ A → B ∧ i∶ B → A ∧ (i o m) = id A ⇒ is_mono m*)
+
+val post_inv_mono = proved_th $
+e0
+(repeat strip_tac >> match_mp_tac ismono_applied >> repeat strip_tac >>
+by_tac (rapf "(i:B->A) o (m:A->B) o (g:X->A) = i o m o h") >-- arw_tac[] >>
+pop_assum mp_tac >> rw_tac[GSYM o_assoc] >> arw_tac[idL] >> strip_tac >> 
+arw_tac[])
+(rapg "!A B m:A->B i:B->A. i o m = id(A) ==> ismono(m)") 
+
+
+(*is_epi f ⇔ ∀g1 g2. dom g1 = dom g2 ∧ cod g1 = cod g2 ∧ dom g1 = cod f ∧ g1 o f = g2 o f ⇒ g1 = g2*)
+
+val _ = new_pred "isepi" [("e",mk_ar_sort (mk_ob "A") (mk_ob "B"))]
+
+val isepi_def = read_axiom "!A B e:A->B. isepi(e) <=> !X f:B->X g. f o e = g o e ==> f = g"
+
+val isepi_applied = isepi_def |> iffRL
+
+val isepi_property = isepi_def |> iffLR 
+
+(*∀A B e i. e∶ A → B ∧ i∶ B → A ∧ e o i = id B ⇒ is_epi e*)
+
+val pre_inv_epi = proved_th $
+e0
+(repeat strip_tac >> match_mp_tac isepi_applied >> repeat strip_tac >>
+by_tac (rapf "(f:B->X) o (e:A->B) o (i:B->A) = g o e o i") >-- arw_tac[GSYM o_assoc] >>
+pop_assum mp_tac >> arw_tac[idR])
+(rapg "!A B e:A->B i:B->A. e o i = id(B) ==> isepi(e)") 
+
+(*is_pb P p q f g <=> cod f = cod g /\ p∶ P → dom f ∧ q∶ P → dom g /\
+                      f o p = g o q ∧
+                      (∀A u v. u∶ A → dom f ∧ v∶ A → dom g ∧ f o u = g o v ⇒
+                      ∃!a. a∶ A → P ∧ p o a = u ∧ q o a = v)*)
+
+val _ = new_pred "ispb" [("f",mk_ar_sort (mk_ob "X") (mk_ob "Z")),
+                         ("g",mk_ar_sort (mk_ob "Y") (mk_ob "Z")),
+                         ("p",mk_ar_sort (mk_ob "P") (mk_ob "X")),
+                         ("q",mk_ar_sort (mk_ob "P") (mk_ob "Y"))]
+
+val ispb_def = read_axiom "!X Z f:X->Z Y g:Y->Z P p:P->X q:P ->Y. ispb(f,g,p,q) <=> f o p = g o q & (!A u:A->X v:A->Y. f o u = g o v ==> ?a: A ->P. !a':A->P. p o a' = u & q o a' = v <=> a' = a)"
+
+(*∀A B f g.
+         f∶A → B ∧ g∶A → B ⇒ f ∘ eqa f g = g ∘ eqa f g*)
+
+val eq_equality = eqind_def |> strip_all_and_imp |> conjE1 |> disch_all |> gen_all
+
+val coeq_equality = coeqind_def |> strip_all_and_imp |> conjE1 |> disch_all |> gen_all
+
+(*f A B. f∶ A → B ==> ?ki. ki∶ coeqo f f → B /\ ki o (coeqa f f) = id B*)
+val iscoeq_def = read_axiom "!A B f:A->B g:A->B cE ce:B->cE. iscoeq(ce,f,g) <=> ce o f = ce o g & !X x:B->X. x o f = x o g ==> (?x0:cE ->X. !x0'. x0' o ce = x <=> x0' = x0)"
+
+(*TODO:
+
+A , B , X ,   
+   (f : A -> B), (x : B -> X), (x0' : B -> X)
+   
+   ----------------------------------------------------------------------
+   x0' = x <=> x0' = x
+
+cannot be solved by rw_tac
+
+ rw_tac[frefl (mk_fvar "f0")]
+
+loops
+
+understand why it is finished by strip_tac
+*)
+
+val coeq_of_equal = proved_th $ 
+e0
+(rw_tac[iscoeq_def] >> repeat strip_tac >> exists_tac (rastt "x:B->X") >> 
+ strip_tac >> rw_tac[idR] >> dimp_tac >> strip_tac)
+(rapg "iscoeq(id(B),f:A->B,f:A->B)")
+
+(*∀A B f g. f∶ A → B ∧ g∶ A → B ⇒ is_mono (eqa f g)*)
+
+val is_eqind = eqind_def |> strip_all_and_imp |> conjE2 |> iffLR |> strip_all_and_imp |> disch_all'' 
+
+val is_coeqind = coeqind_def |> strip_all_and_imp |> conjE2 |> iffLR |> strip_all_and_imp |> disch_all'' 
+
+
+
+val eqa_is_mono = proved_th $
+e0 
+(rw_tac[ismono_def] >> repeat strip_tac >> 
+ suffices_tac  (rapf "h:X->E0 = eqind(e0:E0->A0,f0:A0->B0,g0, e0 o h) & g:X->E0 = eqind(e0:E0->A0,f0:A0->B0,g0, e0 o h) ") 
+ >-- (strip_tac >> once_arw_tac[] >> rw_tac[]) >> 
+ drule eq_equality >> 
+ strip_tac (* 2 *)
+ >> (match_mp_tac (irule_canon is_eqind) >> arw_tac[] >> arw_tac[GSYM o_assoc])
+ )
+(rapg "iseq(e0:E0->A0,f0:A0->B0,g0) ==> ismono(e0)")
+
+(*∀A B f g. f∶ A → B ∧ g∶ A → B ⇒ is_epi (coeqa f g)*)
+
+
+val eqa_is_mono = proved_th $
+e0 
+(rw_tac[isepi_def] >> repeat strip_tac >> 
+ suffices_tac  (rapf "f:cE0->X = coeqind(ce0:B0->cE0,f0:A0->B0,g0, g o ce0) & g:cE0->X = coeqind(ce0:B0->cE0,f0:A0->B0,g0, g o ce0)") 
+ >-- (strip_tac >> once_arw_tac[] >> rw_tac[]) >> 
+ drule coeq_equality >> 
+ strip_tac (* 2 *)
+ >> (match_mp_tac (irule_canon is_coeqind) >> arw_tac[o_assoc]) 
+ )
+(rapg "iscoeq(ce0:B0->cE0,f0:A0->B0,g0) ==> isepi(ce0)")
 
 rapf "!p1AN:AN->A p2AN:AN->N. "
 ∀g h A B. g∶ A → B ∧ h∶ (po (po A N) B) → B ⇒
